Remembered to push...

isabelle/RGA_Relational_Rules.thy
@@ -1,24 +1,24 @@
 theory RGA_Relational_Rules
-  imports Main "~~/src/HOL/Library/Cardinality"
+  imports Main
 begin
 
 datatype 'eid operation
   = MakeList
-  | Insert "'eid option" "'eid"
+  | Insert "'eid"
 
-type_synonym 'eid database = "'eid operation set"
+type_synonym 'eid database = "'eid \<rightharpoonup> 'eid operation"
 
-definition insert :: "'eid::{linorder, card_UNIV} database \<Rightarrow> 'eid option \<Rightarrow> 'eid \<Rightarrow> bool" where
-  "insert \<D> parent i \<longleftrightarrow> Insert parent i \<in> \<D>"
+definition insert :: "'eid::{linorder} database \<Rightarrow> 'eid \<Rightarrow> 'eid \<Rightarrow> bool" where
+  "insert \<D> parent i \<longleftrightarrow> \<D> i = Some (Insert parent)"
 
-inductive list_elem    :: "'eid::{linorder, card_UNIV} database \<Rightarrow> 'eid \<Rightarrow> bool"
-  and has_child        :: "'eid::{linorder, card_UNIV} database \<Rightarrow> 'eid option \<Rightarrow> bool"
-  and child            :: "'eid::{linorder, card_UNIV} database \<Rightarrow> 'eid option \<Rightarrow> 'eid \<Rightarrow> bool"
-  and later_child      :: "'eid::{linorder, card_UNIV} database \<Rightarrow> 'eid option \<Rightarrow> 'eid \<Rightarrow> bool"
-  and sibling          :: "'eid::{linorder, card_UNIV} database \<Rightarrow> 'eid \<Rightarrow> 'eid \<Rightarrow> bool"
-  and later_sibling    :: "'eid::{linorder, card_UNIV} database \<Rightarrow> 'eid \<Rightarrow> 'eid \<Rightarrow> bool"
-  and later_sibling_2  :: "'eid::{linorder, card_UNIV} database \<Rightarrow> 'eid \<Rightarrow> 'eid \<Rightarrow> bool"
-  and has_next_sibling :: "'eid::{linorder, card_UNIV} database \<Rightarrow> 'eid \<Rightarrow> bool"
+inductive list_elem    :: "'eid::{linorder} database \<Rightarrow> 'eid \<Rightarrow> bool"
+  and has_child        :: "'eid::{linorder} database \<Rightarrow> 'eid \<Rightarrow> bool"
+  and child            :: "'eid::{linorder} database \<Rightarrow> 'eid \<Rightarrow> 'eid \<Rightarrow> bool"
+  and later_child      :: "'eid::{linorder} database \<Rightarrow> 'eid \<Rightarrow> 'eid \<Rightarrow> bool"
+  and sibling          :: "'eid::{linorder} database \<Rightarrow> 'eid \<Rightarrow> 'eid \<Rightarrow> bool"
+  and later_sibling    :: "'eid::{linorder} database \<Rightarrow> 'eid \<Rightarrow> 'eid \<Rightarrow> bool"
+  and later_sibling_2  :: "'eid::{linorder} database \<Rightarrow> 'eid \<Rightarrow> 'eid \<Rightarrow> bool"
+  and has_next_sibling :: "'eid::{linorder} database \<Rightarrow> 'eid \<Rightarrow> bool"
 where
   "\<lbrakk>insert \<D> parent i\<rbrakk> \<Longrightarrow> list_elem \<D> i" |
   "\<lbrakk>insert \<D> parent c\<rbrakk> \<Longrightarrow> has_child \<D> parent" |
@@ -29,39 +29,91 @@ where
   "\<lbrakk>sibling \<D> p n; sibling \<D> p l; l < n; n < p\<rbrakk> \<Longrightarrow> later_sibling_2 \<D> p l" |
   "\<lbrakk>later_sibling \<D> p n\<rbrakk> \<Longrightarrow> has_next_sibling \<D> p"
 
-inductive first_child :: "'eid::{linorder, card_UNIV} database \<Rightarrow> 'eid option \<Rightarrow> 'eid \<Rightarrow> bool"
-  and next_sibling    :: "'eid::{linorder, card_UNIV} database \<Rightarrow> 'eid \<Rightarrow> 'eid \<Rightarrow> bool"
-  and siblingless_anc :: "'eid::{linorder, card_UNIV} database \<Rightarrow> 'eid \<Rightarrow> 'eid \<Rightarrow> bool"
-  and next_elem       :: "'eid::{linorder, card_UNIV} database \<Rightarrow> 'eid \<Rightarrow> 'eid \<Rightarrow> bool"
+inductive first_child :: "'eid::{linorder} database \<Rightarrow> 'eid \<Rightarrow> 'eid \<Rightarrow> bool"
+  and next_sibling    :: "'eid::{linorder} database \<Rightarrow> 'eid \<Rightarrow> 'eid \<Rightarrow> bool"
+  and siblingless_anc :: "'eid::{linorder} database \<Rightarrow> 'eid \<Rightarrow> 'eid \<Rightarrow> bool"
+  and next_elem       :: "'eid::{linorder} database \<Rightarrow> 'eid \<Rightarrow> 'eid \<Rightarrow> bool"
 where
   "\<lbrakk>child \<D> parent c; \<not> later_child \<D> parent c\<rbrakk> \<Longrightarrow> first_child \<D> parent c" |
   "\<lbrakk>later_sibling \<D> p n; \<not> later_sibling_2 \<D> p n\<rbrakk> \<Longrightarrow> next_sibling \<D> p n" |
   "\<lbrakk>list_elem \<D> s; \<not> has_next_sibling \<D> s\<rbrakk> \<Longrightarrow> siblingless_anc \<D> s s" |
-  "\<lbrakk>siblingless_anc \<D> s p; child \<D> (Some n) p; \<not> has_next_sibling \<D> n\<rbrakk> \<Longrightarrow> siblingless_anc \<D> s n" |
-  "\<lbrakk>first_child \<D> (Some p) n\<rbrakk> \<Longrightarrow> next_elem \<D> p n" |
-  "\<lbrakk>list_elem \<D> p; \<not> has_child \<D> (Some p); next_sibling \<D> p n\<rbrakk> \<Longrightarrow> next_elem \<D> p n" |
-  "\<lbrakk>list_elem \<D> p; \<not> has_child \<D> (Some p); siblingless_anc \<D> p a; child \<D> (Some p) a; next_sibling \<D> p n\<rbrakk> \<Longrightarrow> next_elem \<D> p n"  
+  "\<lbrakk>siblingless_anc \<D> s p; child \<D> n p; \<not> has_next_sibling \<D> n\<rbrakk> \<Longrightarrow> siblingless_anc \<D> s n" |
+  "\<lbrakk>first_child \<D> p n\<rbrakk> \<Longrightarrow> next_elem \<D> p n" |
+  "\<lbrakk>list_elem \<D> p; \<not> has_child \<D> p; next_sibling \<D> p n\<rbrakk> \<Longrightarrow> next_elem \<D> p n" |
+  "\<lbrakk>list_elem \<D> p; \<not> has_child \<D> p; siblingless_anc \<D> p a; child \<D> p a; next_sibling \<D> p n\<rbrakk> \<Longrightarrow> next_elem \<D> p n"  
 
 lemmas rga_intros [intro] =
   list_elem_has_child_child_later_child_sibling_later_sibling_later_sibling_2_has_next_sibling.intros
   first_child_next_sibling_siblingless_anc_next_elem.intros
+  
+inductive list_iter :: "'eid::{linorder} database \<Rightarrow> 'eid \<Rightarrow> 'eid list \<Rightarrow> bool" where
+  "list_iter \<D> pa []" |
+  "\<lbrakk>first_child \<D> pa e\<rbrakk> \<Longrightarrow> list_iter \<D> pa [e]" |
+  "\<lbrakk>list_iter \<D> pa (e'#es); next_elem \<D> e e'\<rbrakk> \<Longrightarrow> list_iter \<D> pa (e#e'#es)"
 
 lemma first_child_unique:
   assumes "first_child \<D> parent child1"
-  assumes "first_child \<D> parent child2"
+  and "first_child \<D> parent child2"
   shows "child1 = child2"
-by (meson assms rga_intros first_child.cases not_less_iff_gr_or_eq)
+by(meson assms rga_intros first_child.cases not_less_iff_gr_or_eq)
 
 lemma next_sibling_unique:
   assumes "next_sibling \<D> prev next1"
-  assumes "next_sibling \<D> prev next2"
+  and "next_sibling \<D> prev next2"
   shows "next1 = next2"
-by (meson assms rga_intros later_sibling.cases next_sibling.cases not_less_iff_gr_or_eq)
+by(meson assms rga_intros later_sibling.cases next_sibling.cases not_less_iff_gr_or_eq)
 
 lemma next_elem_unique:
   assumes "next_elem \<D> prev next1"
-  assumes "next_elem \<D> prev next2"
+  and "next_elem \<D> prev next2"
   shows "next1 = next2"
-  oops
+sorry
+    
+lemma
+  shows "insert \<D> pa e \<longleftrightarrow> (\<exists>l. e \<in> set l \<and> list_iter \<D> pa l)"
+proof
+  assume "insert \<D> pa e"
+  show "\<exists>l. e \<in> set l \<and> list_iter \<D> pa l"
+    sorry
+next
+  assume "\<exists>l. e \<in> set l \<and> list_iter \<D> pa l"
+  from this obtain l where "list_iter \<D> pa l" and "e \<in> set l"
+    by blast
+  thus "insert \<D> pa e"
+  proof(induction rule: list_iter.induct)
+    fix \<D> pa
+    assume "e \<in> set []"
+    thus "insert \<D> pa e"
+      by auto
+  next
+    fix \<D> pa ea
+    assume "first_child \<D> pa ea" and "e \<in> set [ea]"
+    hence "e = ea"
+      by auto
+    also have "child \<D> pa ea"
+      using \<open>first_child \<D> pa ea\<close> first_child.cases by blast+
+    thus "insert \<D> pa e"
+      using insert_def child.cases \<open>e = ea\<close> by blast
+  next
+    fix \<D> pa e' es ea
+    assume "list_iter \<D> pa (e' # es)"
+      and "e \<in> set (e' # es) \<Longrightarrow> insert \<D> pa e"
+      and "next_elem \<D> ea e'"
+      and "e \<in> set (ea # e' # es)"
+    hence "e = ea \<or> e \<in> set (e'#es)"
+      by auto
+    {
+      assume "e = ea"
+      hence "next_elem \<D> e e'"
+        using \<open>next_elem \<D> ea e'\<close> by auto
+      have "insert \<D> pa e"
+        sorry
+    }
+    thus "insert \<D> pa e"
+      using \<open>e = ea \<or> e \<in> set (e'#es)\<close> \<open>e \<in> set (e' # es) \<Longrightarrow> insert \<D> pa e\<close> by blast
+  qed
+qed
+  
+
 
 end
